Define CyclicityPrefix

ExistentialRules/ChaseSequence/Nontermination/CyclicityPrefix.lean
@@ -7,6 +7,7 @@ module
 
 public import ExistentialRules.ChaseSequence.Nontermination.RepeatableUnblockability
 public import ExistentialRules.ChaseSequence.Termination.Basic
+public import ExistentialRules.Terms.Cyclic
 
 /-!
 # Cyclicity Prefixes
@@ -26,18 +27,95 @@ abbrev Signature.withFreshConstants (sig : Signature) (Fresh : Type u) : Signatu
   C := Sum sig.C Fresh
 }
 
+instance {sig : Signature} {Fresh : Type u} [Inhabited sig.C] : Inhabited (sig.withFreshConstants Fresh).C where
+  default := .inl default
+
 /-- In particular, we can simply use the variables as fresh constants. Think of this as constants that just happen to have the same name as the variables. -/
 abbrev Signature.withFreshConstantsForVars (sig : Signature) : Signature := sig.withFreshConstants sig.V
 
 variable {sig : Signature} [DecidableEq sig.P] [DecidableEq sig.C] [DecidableEq sig.V]
 
 /-- This turns a `VarOrConst` into the constant Sum type of `Signature.withFreshConstants`. -/
-def VarOrConst.cast_withFreshConstantsForVars : TermMapping (VarOrConst sig) sig.withFreshConstantsForVars.C
+def VarOrConst.toConst_withFreshConstantsForVars : TermMapping (VarOrConst sig) sig.withFreshConstantsForVars.C
 | .const c => .inl c
 | .var v => .inr v
+
+/-- Change the constant of a `VarOrConst` into the Sum type of `Signature.withFreshConstants`. -/
+def VarOrConst.cast_withFreshConstantsForVars : TermMapping (VarOrConst sig) (VarOrConst sig.withFreshConstantsForVars)
+| .const c => .const (.inl c)
+| .var v => .var v
+
+/-- Change the constant of a `Rule` into the Sum type of `Signature.withFreshConstants`. -/
+def Rule.cast_withFreshConstantsForVars (r : Rule sig) : Rule sig.withFreshConstantsForVars where
+  body := VarOrConst.cast_withFreshConstantsForVars.apply_generalized_atom_list r.body
+  head := r.head.map VarOrConst.cast_withFreshConstantsForVars.apply_generalized_atom_list
+
+/-- Change the constant of a `RuleSet` into the Sum type of `Signature.withFreshConstants`. -/
+def RuleSet.cast_withFreshConstantsForVars (rs : RuleSet sig) : RuleSet sig.withFreshConstantsForVars :=
+  rs.map Rule.cast_withFreshConstantsForVars
 
 /-- The `body_database` of a rule is the body where each variable is replaced by a fresh constant.
 We achieve this by extending the signature and mapping all terms in the body using `VarOrConst.cast_withFreshConstantsForVars`. -/
 def Rule.body_database (r : Rule sig) : Database sig.withFreshConstantsForVars :=
-  ⟨(VarOrConst.cast_withFreshConstantsForVars.apply_generalized_atom_list r.body).toSet, List.finite_toSet _⟩
+  ⟨(VarOrConst.toConst_withFreshConstantsForVars.apply_generalized_atom_list r.body).toSet, List.finite_toSet _⟩
+
+/-- The trigger for a rule that matches its `body_database`. -/
+def Rule.body_database_trigger (r : Rule sig) : PreTrigger sig.withFreshConstantsForVars where
+  rule := r.cast_withFreshConstantsForVars
+  subs := .const ∘ .inr
+
+/-- For a signature `withFreshConstantsForVars`, we can turn a `GroundSubstitution` into a `ConstantMapping`. -/
+def GroundSubstitution.toConstantMapping_for_sig_withFreshConstantsForVars (subs : GroundSubstitution sig.withFreshConstantsForVars) :
+    ConstantMapping sig.withFreshConstantsForVars
+| .inl c => .const (.inl c) -- we leave original constants untouched
+| .inr v => subs v
+
+/-- We define a structure, which is almost a `CyclicityPrefix` (missing a few conditions). We do this mainly to add some auxiliary definitions that we can use to express the remaining conditions more easily. -/
+structure PreCyclicityPrefix [Inhabited sig.C] (obs : ObsolescenceCondition sig.withFreshConstantsForVars) (rules : RuleSet sig) (hc : HeadChoice sig.withFreshConstantsForVars) (rule : Rule sig)
+    extends RegularChaseDerivationSkeleton obs rules.cast_withFreshConstantsForVars where
+  -- the first conditions are also found in the `CyclicityDerivation`; `growing` and `unblockable` are missing though
+  adheres_to_headChoice : ChaseDerivationSkeleton.adheres_to_headChoice toChaseDerivationSkeleton hc
+  triggers_loaded : ∀ cd2, cd2 <:+ toChaseDerivationSkeleton -> ∀ next ∈ cd2.next, ∃ orig ∈ next.origin, orig.fst.val.loaded cd2.head.facts
+  -- from here things are different
+  finite : toChaseDerivationSkeleton.terminates
+  first_trigger : ∃ orig, ∃ (orig_mem : orig ∈ toChaseDerivationSkeleton.head.origin),
+    orig.fst.val = rule.body_database_trigger ∧
+    orig.fst.val.unblockable rules.cast_withFreshConstantsForVars hc ∧
+    toChaseDerivationSkeleton.head.facts = rule.body_database.toFactSet.val ∪ (RegularChaseNode.regularChaseNodeInstance.origin_result toChaseDerivationSkeleton.head (by simp only [ChaseNode.origin]; rw [orig_mem]; simp)).toSet
+
+namespace PreCyclicityPrefix
+
+variable [Inhabited sig.C] {obs : ObsolescenceCondition sig.withFreshConstantsForVars} {rules : RuleSet sig} {hc : HeadChoice sig.withFreshConstantsForVars} {rule : Rule sig}
+
+/-- Every node in the `PreCyclicityPrefix` must have an origin. -/
+theorem isSome_origin_of_mem {cd : PreCyclicityPrefix obs rules hc rule} : ∀ node ∈ cd.toChaseDerivationSkeleton, node.origin.isSome := by
+  intro node node_mem
+  rw [cd.mem_iff_eq_head_or_mem_tail] at node_mem
+  cases node_mem with
+  | inl node_mem => rw [node_mem]; rcases cd.first_trigger with ⟨orig, orig_mem, _⟩; rw [orig_mem]; simp
+  | inr node_mem => simp only [cd.mem_tail_iff] at node_mem; rcases node_mem with ⟨_, cd2, suf, mem⟩; apply cd2.isSome_origin_next; exact mem
+
+/-- Obtain the origin of a node (which must exist). -/
+def origin_of_mem {cd : PreCyclicityPrefix obs rules hc rule} {node : RegularChaseNode obs rules.cast_withFreshConstantsForVars}
+    (node_mem : node ∈ cd.toChaseDerivationSkeleton) :=
+  node.origin.get (cd.isSome_origin_of_mem node node_mem)
+
+/-- The origin of the last node (the prefix is finite). -/
+def last_origin (cd : PreCyclicityPrefix obs rules hc rule) := cd.origin_of_mem (cd.last_mem cd.finite)
+
+/-- In the end, we want to repeat the prefix using a constant mapping expressing the mapping from the first to the last trigger. This mapping is what is defined here. -/
+def constantMappingForRepetition (cd : PreCyclicityPrefix obs rules hc rule) : ConstantMapping sig.withFreshConstantsForVars :=
+  cd.last_origin.fst.val.subs.toConstantMapping_for_sig_withFreshConstantsForVars
+
+end PreCyclicityPrefix
+
+/-- The actual `CyclicityPrefix` extending the `PreCyclicityPrefix` with the remaining conditions. -/
+structure CyclicityPrefix [Inhabited sig.C] (obs : ObsolescenceCondition sig.withFreshConstantsForVars) (unblk : RepeatableUnblockability obs) (rules : RuleSet sig) (hc : HeadChoice sig.withFreshConstantsForVars) (rule : Rule sig)
+    extends PreCyclicityPrefix obs rules hc rule where
+  -- NOTE: we only demand unblockability on all triggers but the first one. This is indeed correct and necessary.
+  triggers_unblockable : ∀ h, ∀ node ∈ toChaseDerivationSkeleton.tail h, ∀ orig ∈ node.origin, unblk.trigger_unblockable rules.cast_withFreshConstantsForVars hc orig.fst.val
+  last_trigger : toPreCyclicityPrefix.last_origin.fst.val.rule = rule.cast_withFreshConstantsForVars ∧ ∃ term ∈ (toPreCyclicityPrefix.last_origin.fst.val.output_for_headChoice hc).flatMap GeneralizedAtom.terms, PreGroundTerm.ruleCyclic rule.cast_withFreshConstantsForVars term.val
+  constantMapping_reversible_in_each_step : ∀ h, ∀ node ∈ toChaseDerivationSkeleton.tail h, ∀ orig ∈ node.origin, ∀ j : Nat,
+    toPreCyclicityPrefix.constantMappingForRepetition.isReversible
+      {rule := orig.fst.val.rule, subs := (toPreCyclicityPrefix.constantMappingForRepetition.apply_ground_term.repeat_fun j) ∘ orig.fst.val.subs : PreTrigger _}.termSkeleton.toSet
 
